Mostly cleaned up Bookstore.

ADTExamples/QueryStructure/Bookstore.v
@@ -1,56 +1,52 @@
-Require Import String Omega List FunctionalExtensionality Ensembles.
-
-Ltac typeof' pf := type of pf.
-Ltac simpl_typeof pf := cbv delta in (type of pf).
-
-Require Import Computation ADT ADTRefinement ADT.Pick
-        ADTRefinement.BuildADTRefinements ADTNotation
-        QueryStructureSchema QueryQSSpecs InsertQSSpecs QueryStructure.
-
-Generalizable All Variables.
-Set Implicit Arguments.
+Require Import String Omega List FunctionalExtensionality Ensembles
+        Computation ADT ADTRefinement ADTNotation QueryStructureSchema
+        BuildADTRefinements QueryQSSpecs InsertQSSpecs
+        QueryStructure GeneralInsertRefinements ListInsertRefinements
+        GeneralQueryRefinements ListQueryRefinements
+        ProcessScheduler.AdditionalLemmas.
 
 Section BookStoreExamples.
 
-  Arguments Tuple [Heading] .
-  Arguments BoundedString [_].
-
   (* Our bookstore has two relations (tables):
-     - The books in the inventory
-     - The orders that have been placed *)
+     - The [Books] relation contains the books in the
+       inventory, represented as a tuple with
+       [Author], [Title], and [ISBN] attributes.
+       The [ISBN] attribute is a key for the relation,
+       specified by the [where attributes .. depend on ..]
+       constraint.
+     - The [Orders] relation contains the orders that
+       have been placed, represented as a tuple with the
+       [ISBN] and [Date] attributes.
 
-Open Scope QSSchema.
+     The schema for the entire query structure specifies that
+     the [ISBN] attribute of [Orders] is a foreign key into
+     [Books], specified by the [attribute .. of .. references ..]
+     constraint.
+   *)
+
+  Open Scope QSSchema.
 
   Definition BookStoreSchema :=
     query structure schema
       [ relation "Books" has
-                schema <"Author" : string,
-                        "Title" : string,
-                        "ISBN" : nat>
+                schema <"Author" :: string,
+                        "Title" :: string,
+                        "ISBN" :: nat>
                 where attributes ["Title"; "Author"] depend on ["ISBN"];
         relation "Orders" has
-                schema <"ISBN" : nat,
-                        "Date" : nat> ]
+                schema <"ISBN" :: nat,
+                        "Date" :: nat> ]
       enforcing [attribute "ISBN" of "Orders" references "Books"].
 
-Definition Books := GetRelationKey BookStoreSchema "Books".
-Definition Orders := GetRelationKey BookStoreSchema "Orders".
+  Definition Books := GetRelationKey BookStoreSchema "Books".
+  Definition Orders := GetRelationKey BookStoreSchema "Orders".
 
-Definition Author := GetAttributeKey Books "Author".
-Definition Title := GetAttributeKey Books "Title".
-Definition ISBN := GetAttributeKey Books "ISBN".
+  Definition Author := GetAttributeKey Books "Author".
+  Definition Title := GetAttributeKey Books "Title".
+  Definition ISBN := GetAttributeKey Books "ISBN".
 
-Definition oISBN := GetAttributeKey Orders "ISBN".
-Definition Date := GetAttributeKey Orders "Date".
-
-
-  (* Sanity check to show that the definitions produced
-     can be efficiently evaluated. *)
-  Goal (forall b,
-          BuildQueryStructureConstraints
-            BookStoreSchema Orders Books = b).
-  Time simpl.
-  Abort.
+  Definition oISBN := GetAttributeKey Orders "ISBN".
+  Definition Date := GetAttributeKey Orders "Date".
 
   Definition BookStoreRefRep := QueryStructure BookStoreSchema.
 
@@ -75,38 +71,34 @@ Definition Date := GetAttributeKey Orders "Date".
   Local Open Scope QueryStructureParsing_scope.
   Local Open Scope Schema.
   Local Open Scope QuerySpec.
-
-  Definition PlaceOrder := "P"%string.
-  Definition AddBook := "A"%string.
-  Definition GetTitles := "G"%string.
-  Definition NumOrders := "N"%string.
+  Local Open Scope string.
 
   Definition BookStoreSig : ADTSig :=
     ADTsignature {
-        PlaceOrder : rep × Order → rep,
-        AddBook : rep × Book → rep ;
-        GetTitles : rep × string → list string,
-        NumOrders : rep × string → nat
+        "PlaceOrder" : rep × Order → rep,
+        "AddBook" : rep × Book → rep ;
+        "GetTitles" : rep × string → list string,
+        "NumOrders" : rep × string → nat
       }.
 
   Definition BookStoreSpec : ADT BookStoreSig :=
     QueryADTRep BookStoreRefRep {
              (* [PlaceOrder] : Place an order into the 'Orders' table *)
-                  def update PlaceOrder ( o : Order ) : rep :=
+                  def update "PlaceOrder" ( o : Order ) : rep :=
                     Insert o into Orders,
 
              (* [AddBook] : Add a book to the inventory *)
-             def update AddBook ( b : Book ) : rep :=
+             def update "AddBook" ( b : Book ) : rep :=
                  Insert b into Books ;
 
              (* [GetTitles] : The titles of books written by a given author *)
-             def query GetTitles ( author : string ) : list string :=
+             def query "GetTitles" ( author : string ) : list string :=
                For (b in Books)
                Where (author = b!Author)
                Return (b!Title),
 
              (* [NumOrders] : The number of orders for a given author *)
-             def query NumOrders ( author : string ) : nat :=
+             def query "NumOrders" ( author : string ) : nat :=
                  Count (For (o in Orders) (b in Books)
                         Where (author = b!Author)
                         Where (b!ISBN = o!oISBN)
@@ -117,442 +109,117 @@ Definition Date := GetAttributeKey Orders "Date".
   Local Close Scope QuerySpec.
   Local Open Scope QueryStructure_scope.
 
-  Open Scope updateDef.
-
-  Require Import ProcessScheduler.AdditionalLemmas SetEq.
-
-  Lemma refine_SetEq_self {A} :
-    forall l : list A,
-      refine {l' | SetEq l' l}%comp
-             (ret l).
-  Proof.
-    unfold SetEq, refine; intros; inversion_by computes_to_inv.
-    econstructor; subst; split; eauto.
-  Qed.
-
-  Definition Equivalent_Ensembles {A : Type}
-             (P Q : Ensemble A) := forall a, P a <-> Q a.
-
-  Lemma Equivalent_In_EnsembleListEquivalence {A}
-        (qs : QueryStructureHint) (R : _)
-        (l : list _)
-        bod
-  : EnsembleListEquivalence (GetRelation qsHint R) l ->
-    Equivalent_Ensembles
-      (@Query_In qs A R bod)
-      (fun a => exists tup, List.In tup l /\ bod tup a).
-  Proof.
-    split; intros; unfold In in *.
-    destruct H0; eexists; intuition; eauto.
-    eapply H; eauto.
-    destruct H0; intuition; eexists; split; eauto.
-    eapply H; eauto.
-  Qed.
-
-  Definition Join_Lists {A B}
-             (l : list A)
-             (l' : list B)
-  : list (A * B) :=
-    fold_left (@app _) (map (fun a => map (fun b => (a, b)) l') l) nil.
-
-  Lemma In_fold_left_app {A}
-  : forall (l : list (list A))
-           (l'' : list A)
-           (a : A),
-      List.In a (fold_left (@app _) l l'') <->
-      (List.In a l'' \/ (exists l', List.In l' l /\ List.In a l')).
-  Proof.
-    induction l; simpl; intuition.
-    destruct_ex; intuition.
-    destruct (proj1 (IHl _ _) H).
-    apply in_app_or in H0; intuition; eauto.
-    destruct_ex; intuition; eauto.
-    eapply IHl; eauto using in_or_app.
-    destruct_ex; intuition; subst; eauto.
-    eapply IHl; eauto using in_or_app.
-    eapply IHl; eauto using in_or_app.
-  Qed.
-
-  Lemma In_Join_Lists {A B}
-  : forall (l : list A)
-           (l' : list B)
-           (a : A)
-           (b : B),
-      List.In (a, b) (Join_Lists l l') <->
-      (List.In a l /\ List.In b l').
-  Proof.
-    unfold Join_Lists; split; intros.
-    apply In_fold_left_app in H; simpl in *; intuition;
-    destruct_ex; intuition;
-    apply in_map_iff in H0; destruct_ex; intuition; subst;
-    apply in_map_iff in H1; destruct_ex; intuition; subst;
-    simpl; congruence.
-    intuition.
-    apply In_fold_left_app; right.
-    exists (map (fun b : B => (a, b)) l'); split;
-    apply in_map_iff; eexists; intuition; eauto.
-  Qed.
-
-  Lemma Equivalent_Join_Lists {A B}
-        (qs : QueryStructureHint) (R : _)
-        (l : list B)
-        (l' : list _)
-        bod
-  : EnsembleListEquivalence (GetRelation qsHint R) l' ->
-    Equivalent_Ensembles
-      (fun a => exists b, List.In b l /\
-                            (@Query_In qs A R (bod b) a))
-      (fun a => exists b, List.In b (Join_Lists l l') /\
-                          (bod (fst b) (snd b) a)).
-  Proof.
-    split; intros; unfold In in *.
-    - destruct H0; intuition; destruct H2; eexists; intuition; eauto.
-      unfold EnsembleListEquivalence in H.
-      apply In_Join_Lists; split; eauto.
-      eapply H; unfold In; apply H2.
-      simpl; auto.
-    - destruct_ex; intuition; destruct x; eexists; intuition.
-      eapply (In_Join_Lists l l'); eauto.
-      unfold Query_In; eexists; intuition; eauto.
-      apply H; eapply (In_Join_Lists l l'); eauto.
-  Qed.
-
-  Lemma Equivalent_List_In_Where {A B}
-        (l : list B)
-        (P : Ensemble B)
-        (bod : B -> Ensemble A)
-        (cond : B -> bool)
-        : (forall a, cond a = true <-> P a)
-          ->
-    Equivalent_Ensembles
-      (fun a : A => exists b, List.In b l /\ Query_Where (P b) (bod b) a)
-      (fun a : A => exists b, List.In b (filter cond l) /\ (bod b) a)
-  .
-  Proof.
-    split; intros; unfold In, Query_Where in *.
-    destruct H0; eexists; intuition; eauto.
-    eapply filter_In; split; eauto.
-    eapply H; eauto.
-    destruct H0; intuition; eexists; split; eauto.
-    eapply filter_In; eauto.
-    intuition; eauto using filter_In.
-    eapply H; eapply filter_In; eauto.
-  Qed.
-
-  Lemma Equivalent_Swap_In {A}
-        (qs : QueryStructureHint) (R R' : _)
-        (bod : Tuple -> Tuple -> Ensemble A)
-  :
-    Equivalent_Ensembles
-      (@Query_In qs _ R (fun tup => @Query_In qs _ R' (bod tup)))
-      (@Query_In qs _ R' (fun tup => @Query_In qs _ R
-                                               (fun tup' => bod tup' tup))).
-  Proof.
-    unfold Equivalent_Ensembles, Query_In; split; intros;
-    repeat (progress (destruct_ex; intuition)); eexists;
-    split; eauto.
-  Qed.
-
-  Lemma Equivalent_Swap_In_Where {A}
-        (qs : QueryStructureHint) (R : _)
-        {heading}
-        (bod : @Tuple heading -> Tuple -> Ensemble A)
-        (P : @Tuple heading -> Prop)
-  :
-    pointwise_relation
-      Tuple Equivalent_Ensembles
-      (fun tup' : Tuple =>
-         (@Query_In qs _ R
-                    (fun tup => Query_Where (P tup') (bod tup' tup))))
-      (fun tup' : Tuple =>
-         Query_Where (P tup') (@Query_In qs _ R (bod tup'))).
-  Proof.
-    unfold Equivalent_Ensembles, Query_In, Query_Where; split; intros;
-    repeat (progress (destruct_ex; intuition)); eexists;
-    split; eauto.
-  Qed.
-
-  Lemma refine_For_List_Return {A B}
-        (l : list B)
-        (extract : B -> A)
-  : refine
-      (For (fun a : A =>
-              exists b : B,
-                List.In b l /\ Return (extract b) a))%QuerySpec
-      (ret (map extract l)).
-  Proof.
-    unfold refine; intros; inversion_by computes_to_inv; subst.
-    econstructor; unfold In, Query_Return; split; intros.
-    eapply in_map_iff in H; destruct_ex; intuition; eauto.
-    eapply in_map_iff; destruct_ex; intuition; eauto.
-  Qed.
-
-  Add Parametric Morphism {A: Type} :
-    (Query_For)
-      with signature (@Equivalent_Ensembles A ==> refine)
-        as refine_Query_For_Equivalent.
-  Proof.
-    unfold impl, Query_For, refine; intros.
-    inversion_by computes_to_inv.
-    econstructor; split_iff; split; intros; eauto.
-    apply H; apply H1; auto.
-    apply H2; apply H; auto.
-  Qed.
-
-  Add Parametric Morphism {A: Type}
-      (qs : QueryStructureHint) (R : _)
-  :
-    (fun bod => Query_For (@Query_In qs _ R bod))
-      with signature ((pointwise_relation Tuple (@Equivalent_Ensembles A) ==> refine ))
-        as refine_Query_For_In_Equivalent.
-  Proof.
-    unfold impl, Query_For, pointwise_relation, Query_In, In, refine.
-    intros; inversion_by computes_to_inv.
-    econstructor; split_iff; split; intros; eauto.
-    destruct (H1 _ H0); eexists; intuition; eauto.
-    apply H; auto.
-    destruct_ex; apply H2; eexists; intuition; eauto.
-    apply H; auto.
-  Qed.
-
-  Lemma tupleAgree_refl :
-    forall (h : Heading)
-           (tup : @Tuple h)
-           (attrlist : list (Attributes h)),
-      tupleAgree tup tup attrlist.
-  Proof.
-    unfold tupleAgree; auto.
-  Qed.
-
-  Lemma refine_tupleAgree_refl_True :
-    forall (h : Heading)
-           (tup : @Tuple h)
-           (attrlist attrlist' : list (Attributes h)),
-      refine {b |
-              decides b (tupleAgree tup tup attrlist'
-                         -> tupleAgree tup tup attrlist)}
-             (ret true).
-  Proof.
-    unfold refine; intros; inversion_by computes_to_inv.
-    subst; econstructor; simpl; auto using tupleAgree_refl.
-  Qed.
-
-  Definition decideable_Heading_Domain
-             (h : Heading) :=
-    forall (idx : Attributes h)
-           (t t' : Domain h idx), {t = t'} + {t <> t'}.
-
-  Fixpoint Tuple_Agree_dec
-             (h : Heading)
-             (h_dec_eq : decideable_Heading_Domain h)
-             (attrlist : list (Attributes h))
-  : forall (tup tup' : Tuple),
-      {tupleAgree tup tup' attrlist} + {~tupleAgree tup tup' attrlist}.
-  Proof.
-  Admitted.
-
-  Lemma BookSchemaHeading_dec 
+  Lemma BookSchemaHeading_dec
     : decideable_Heading_Domain BookSchemaHeading.
   Proof.
   Admitted.
 
-  Fixpoint Check_List_Prop {A}
-           (cond : A -> bool)
-           (l : list A)
-  : bool :=
-    match l with
-        | [] => true
-        | a :: l' => if (cond a) then
-                          Check_List_Prop cond l'
-                        else false
-    end.
-
-  Definition In_List_Key 
-           (h : Heading)
-           (h_dec_eq : decideable_Heading_Domain h)
-           (attrlist : list (Attributes h))
-           (tup : Tuple)
-           (l : list Tuple) :=
-    Check_List_Prop (fun tup' => 
-                       if (Tuple_Agree_dec h_dec_eq attrlist tup tup')
-                       then true
-                       else false) l.
-
-  Lemma refine_unused_key_check
-  : forall (h : Heading)
-           (h_dec_eq : decideable_Heading_Domain h)
-           (attrlist attrlist' : list (Attributes h))
-           (tup : Tuple)
-           (rel : Ensemble Tuple)
-           (l : list Tuple),
-      EnsembleListEquivalence rel l
-      -> refine {b | decides b
-                             (forall tup' : Tuple,
-                                rel tup' ->
-                                tupleAgree tup tup' attrlist' ->
-                                tupleAgree tup tup' attrlist)}
-                (ret (In_List_Key h_dec_eq attrlist tup l)).
-  Admitted.
-
-  Lemma refine_unused_key_check'
-  : forall (h : Heading)
-           (h_dec_eq : decideable_Heading_Domain h)
-           (attrlist attrlist' : list (Attributes h))
-           (tup : Tuple)
-           (rel : Ensemble Tuple)
-           (l : list Tuple),
-      EnsembleListEquivalence rel l
-      -> refine {b | decides b
-                             (forall tup' : Tuple,
-                                rel tup' ->
-                                tupleAgree tup' tup attrlist' ->
-                                tupleAgree tup' tup attrlist)}
-                (ret (In_List_Key h_dec_eq attrlist tup l)).
-  Admitted.
-
-  Lemma refine_foreign_key_check 
-  : forall (h : Heading)
-           (rel : Ensemble Tuple)
-           (l : list Tuple)
-           (P : Ensemble Tuple)
-           (cond : Tuple -> bool),
-      EnsembleListEquivalence rel l
-      -> refine {b  |
-                 decides b
-                         (exists tup' : @Tuple h,
-                            rel tup' /\
-                            P tup')}
-                (ret (Check_List_Prop cond l)).
-    Admitted.
-
-  Lemma refine_pick_eq_ex_bind {A B : Type}
-        (P : A -> B -> Prop)
-        (a : A)
-  : refine (a' <- {a' | a' = a /\ exists b, P a' b};
-            {b | P a' b})
-           {b | P a b}.
-  Proof.
-    unfold refine; intros; inversion_by computes_to_inv;
-    econstructor; eauto.
-  Qed.
-
-  Lemma refine_under_if {A B} 
-        (P : A -> B -> Prop) : 
-    forall (cond : bool) (ta ea : A) ta' ea', 
-      refine {b | P ta b} ta'
-      -> refine {b | P ea b} ea'
-      -> refine {b | P (if cond then ta else ea) b}
-                (if cond then ta' else ea').
-  Proof.
-    intros; destruct cond; eauto.
-  Qed.
-
-  Lemma refine_if_ret {A}
-  : forall (cond : bool) (ta ea : A), 
-      refineEquiv (ret (if cond then ta else ea))
-                  (if cond then ret ta else ret ea).
-  Proof.
-    split; destruct cond; reflexivity.
-  Qed.
-
   Definition BookStoreListImpl_SiR or (nr : (list Book) * (list Order)) : Prop :=
     (EnsembleListEquivalence (GetUnConstrRelation or Books) (fst nr))
     /\ (EnsembleListEquivalence (GetUnConstrRelation or Orders) (snd nr)).
+
+  Definition Refinement_of_method
+             {Rep Dom : Type}
+             (mut : mutatorMethodType Rep Dom)
+    := sigT (fun newDef =>
+               (forall n (r_n : Rep),
+                  refine (mut r_n n)
+                         (newDef r_n n))).
+
+  Lemma Method_Refinement_Step
+        {Rep Dom : Type}
+        (mut : mutatorMethodType Rep Dom)
+        (mut' : sigT (fun mut' => forall n (r_n : Rep),
+                                    refine (mut r_n n)
+                                           (mut' r_n n)))
+  : Refinement_of_method (proj1_sig mut')
+    -> Refinement_of_method mut.
+  Proof.
+    intros H0; exists (proj1_sig H0).
+    intros; etransitivity; eauto.
+    eapply (proj2_sig mut').
+    eapply (proj2_sig H0).
+  Qed.
 
   Definition BookStore :
     Sharpened BookStoreSpec.
   Proof.
     unfold BookStoreSpec.
 
-    hone representation' using (@DropQSConstraints_SiR _).
+    (* Step 1: Drop the constraints on the tables. From the perspective
+      of a client of a sharpened ADT the invariants will still hold,
+      since ADT refinement preserves the simulation relation.   *)
 
-    (* Step 1: Decide what to do when inserting a book that
-       violates the key constraints of Books. I think
-       we will leave table unchanged when a 'bad' book is
-       inserted. *)
-    hone' mutator PlaceOrder.
+    hone representation using (@DropQSConstraints_SiR BookStoreSchema).
+
+    (* Step 2: Remove extraneous schema and cross-relation constraints
+       from the [PlaceOrder] mutator so that subsequent refinements
+       will only need to implement with the foreign key constraint. *)
+
+    hone mutator "PlaceOrder".
     {
-      setoid_rewrite refineEquiv_pick_eq'.
-      simplify with monad laws.
-      apply refine_pick_forall_Prop with
-      (P := fun r_n or (n' : _) => _).
-      intros; setoid_rewrite QSInsertSpec_UnConstr_refine; simpl; eauto.
+      set_evars.
+      intros; setoid_rewrite QSInsertSpec_UnConstr_refine; eauto; simpl.
       setoid_rewrite decides_True.
+      setoid_rewrite decides_2_True.
       setoid_rewrite decides_3_True.
-      (* This takes 24 seconds on my machine.
-         The term size isn't the problem, as non of the goals
-         along the way are particularly large.
-
-         Time (setoid_rewrite refineEquiv_bind_unit;
-         setoid_rewrite refineEquiv_bind_unit;
-         setoid_rewrite refineEquiv_bind_unit;
-         setoid_rewrite refineEquiv_bind_unit) *)
       simplify with monad laws.
       unfold If_Then_Else; simpl.
       setoid_rewrite refine_if_bool_eta.
-      simplify with monad laws.
-      unfold SatisfiesSchemaConstraints; simpl; intros.
-      setoid_rewrite decides_2_True.
       simplify with monad laws.
       finish honing.
     }
-    (* Step 2: Decide what to do when adding an order that
-       violates foreign key constraints of Orders. *)
-    hone' mutator AddBook.
+
+    (* Step 3: Similarly remove extraneous schema and cross-relation
+       constraints [AddBook] mutator so that subsequent refinements
+       will only need to implement the single key constraint. *)
+
+    hone mutator "AddBook".
     {
-      setoid_rewrite refineEquiv_pick_eq'.
-      simplify with monad laws.
-      apply refine_pick_forall_Prop with
-      (P := fun r_n or (n' : _) => _).
-      intros; setoid_rewrite QSInsertSpec_UnConstr_refine; simpl; eauto.
+      set_evars.
+      intros; setoid_rewrite QSInsertSpec_UnConstr_refine; eauto; simpl.
       setoid_rewrite decides_True.
       setoid_rewrite decides_3_True.
-      setoid_rewrite refineEquiv_bind_unit.
-      unfold If_Then_Else; simpl.
-      setoid_rewrite refine_if_bool_eta.
-      simplify with monad laws.
-      unfold SatisfiesSchemaConstraints; simpl; intros.
       rewrite refine_tupleAgree_refl_True.
       simplify with monad laws.
-      remove_trivial_insertion_constraints r_n n Orders Books oISBN ISBN H0.
+      remove_trivial_insertion_constraints r_n n Orders Books
+                                           oISBN ISBN  H.
       finish honing.
     }
 
-    hone representation' using BookStoreListImpl_SiR.
+    (* Step 4: Switch to an implementation of the representation
+       type as a pair of lists of tuples. *)
 
-    (* honing Get Titles. *)
-    hone' observer GetTitles using _.
-    { intros; subst.
-      set_evars; cbv delta [obsCod obsDom observerMethodType] beta in H; simpl in H.
+    hone representation using BookStoreListImpl_SiR.
+
+    (* Step 5: Implement the [GetTitles] observer. *)
+    hone observer "GetTitles".
+    { destruct H; subst; simpl in *.
+      set_evars; simpl in *.
+      rewrite refine_pick_computes_to.
       apply refine_pick_forall_Prop with
-      (P := fun r_n or (n' : list string) => _).
-      intros; rewrite refine_pick_computes_to.
-      apply refine_pick_forall_Prop with
-      (P := fun r_n or (n' : list string) => _).
-      destruct H0; unfold DropQSConstraints_SiR; intros; subst.
+      (P := fun _ _ _ => _); intros.
+      unfold DropQSConstraints_SiR in H2; intros; subst.
       intros; rewrite refine_pick_computes_to.
       repeat rewrite GetRelDropConstraints in *.
       setoid_rewrite Equivalent_In_EnsembleListEquivalence; simpl; eauto.
       setoid_rewrite Equivalent_List_In_Where with
       (cond := fun (a0 : Book) => if (string_dec (GetAttribute a0 Author) n) then true else false); simpl.
       rewrite refine_For_List_Return.
-      unfold H; exact (reflexivity _).
+      finish honing.
       intros; destruct (string_dec (a!Author)%Tuple n); split; intros;
       auto; congruence.
     }
 
-    (* honing Num Orders *)
+    (* Step 5: Implement the [NumOrders] observer. *)
 
-    hone' observer NumOrders using _.
+    hone observer "NumOrders".
     {
-      intros; subst.
-      set_evars; cbv delta [obsCod obsDom observerMethodType] beta in H; simpl in H.
-      apply refine_pick_forall_Prop with
-      (P := fun r_n or (n' : _) => _).
+      destruct H; subst; set_evars; simpl in *.
       intros; rewrite refine_pick_computes_to.
       apply refine_pick_forall_Prop with
       (P := fun r_n or (n' : _) => _).
-      unfold Count, DropQSConstraints_SiR; destruct H0; intros; subst.
+      unfold Count, DropQSConstraints_SiR; intros; subst.
       repeat rewrite GetRelDropConstraints in *.
       rewrite refine_pick_computes_to; eauto.
       rewrite Equivalent_Swap_In.
@@ -572,53 +239,36 @@ Definition Date := GetAttributeKey Orders "Date".
                then true else false); simpl.
     rewrite refine_For_List_Return.
     simplify with monad laws.
-    unfold H; exact (reflexivity _).
+    exact (reflexivity _).
     { intros; destruct (eq_nat_dec ((fst a)!ISBN)%Tuple ((snd a)!oISBN)%Tuple);
       split; intros; auto; congruence. }
     { intros; destruct (string_dec (a!Author)%Tuple n); split; intros;
     auto; congruence. }
     }
 
-    hone' mutator AddBook.
-    {
-      setoid_rewrite refineEquiv_pick_eq'.
-      setoid_rewrite refineEquiv_unit_bind.
-      apply refine_pick_forall_Prop with
-      (P := fun r_n or (b : _)  => _).
+    hone mutator "AddBook".
+    { destruct H; set_evars.
       setoid_rewrite refineEquiv_split_ex.
       setoid_rewrite refineEquiv_pick_computes_to_and.
       simplify with monad laws.
-      unfold SatisfiesSchemaConstraints; simpl; intros.
-      destruct H0.
-      setoid_rewrite refine_unused_key_check with 
+      setoid_rewrite refine_unused_key_check with
       (h_dec_eq := BookSchemaHeading_dec ); eauto.
-      simplify with monad laws. 
+      simplify with monad laws.
       setoid_rewrite refine_unused_key_check' with
       (h_dec_eq := BookSchemaHeading_dec ); eauto.
       simplify with monad laws.
       rewrite refine_pick_eq_ex_bind.
-      rewrite refine_under_if with (ea' := ret r_n); 
+      rewrite refine_under_if with (ea' := ret r_n);
         [ | reflexivity |
-          econstructor; inversion_by computes_to_inv; subst; 
+          econstructor; inversion_by computes_to_inv; subst;
           constructor; eauto] .
-
-
-      Add Parametric Morphism {A: Type} (b : bool):
-        (If_Then_Else b)
-          with signature (
-            @refine A ==> @refine A ==> refine)
-            as refine_refine_if.
-      Proof.
-        unfold refine, If_Then_Else; intros.
-        destruct b; eauto.
-      Qed.
 
       apply refine_refine_if; [ | reflexivity ].
 
-      apply refine_under_if with (ea' := ret r_n); 
-        [ | econstructor; inversion_by computes_to_inv; subst; 
+      apply refine_under_if with (ea' := ret r_n);
+        [ | econstructor; inversion_by computes_to_inv; subst;
           constructor; eauto] .
-      unfold BookStoreListImpl_SiR; 
+      unfold BookStoreListImpl_SiR;
         unfold GetUnConstrRelation, ith_Bounded; simpl.
       erewrite refine_pick with (c := ret (n :: fst r_n, snd r_n)).
       reflexivity.
@@ -626,21 +276,17 @@ Definition Date := GetAttributeKey Orders "Date".
       unfold GetUnConstrRelation, ith_Bounded,
       EnsembleListEquivalence, RelationInsert, In in *; simpl in *;
       split; intuition; eauto.
-      right; eapply H0; eauto.
-      right; eapply H0; eauto.
+      right; eapply H; eauto.
+      right; eapply H; eauto.
     }
 
-    hone' mutator PlaceOrder.
-    {
-      setoid_rewrite refineEquiv_pick_eq'.
-      setoid_rewrite refineEquiv_unit_bind.
-      apply refine_pick_forall_Prop with
-      (P := fun r_n or (b : _)  => _).
+    hone mutator "PlaceOrder".
+    { set_evars.
       setoid_rewrite refineEquiv_split_ex.
       setoid_rewrite refineEquiv_pick_computes_to_and.
       simplify with monad laws.
       intros.
-      destruct H0; rewrite refine_foreign_key_check
+      destruct H; rewrite refine_foreign_key_check
                    with (cond := fun a =>
                                    if (eq_nat_dec (a!ISBN)%Tuple (n!oISBN)%Tuple)
                                    then true
@@ -649,12 +295,12 @@ Definition Date := GetAttributeKey Orders "Date".
 ; eauto.
       simplify with monad laws.
       rewrite refine_pick_eq_ex_bind.
-      rewrite refine_under_if with (ea' := ret r_n); 
+      rewrite refine_under_if with (ea' := ret r_n);
         [ | reflexivity |
-          econstructor; inversion_by computes_to_inv; subst; 
+          econstructor; inversion_by computes_to_inv; subst;
           constructor; eauto] .
       apply refine_refine_if; [ | reflexivity ].
-      unfold BookStoreListImpl_SiR; 
+      unfold BookStoreListImpl_SiR;
         unfold GetUnConstrRelation, ith_Bounded; simpl.
       erewrite refine_pick with (c := ret (fst r_n, n :: snd r_n)).
       reflexivity.
@@ -664,11 +310,11 @@ Definition Date := GetAttributeKey Orders "Date".
       split; intuition; eauto.
       right; eapply H1; eauto.
       right; eapply H1; eauto.
-    }      
+    }
 
     (* Step 4: Profit. :)*)
 
-    finish sharpening. 
+    finish sharpening.
   Defined.
 
     (* Alternate 'simple' steps. *)
