ADTExamples/QueryStructure/GeneralInsertRefinements.v
@@ -1,0 +1,25 @@
+Require Import String Omega List FunctionalExtensionality Ensembles
+        Computation ADT ADTRefinement ADTNotation QueryStructureSchema
+        QueryQSSpecs InsertQSSpecs QueryStructure.
+
+Lemma tupleAgree_refl :
+  forall (h : Heading)
+         (tup : @Tuple h)
+         (attrlist : list (Attributes h)),
+    tupleAgree tup tup attrlist.
+  Proof.
+    unfold tupleAgree; auto.
+  Qed.
+
+  Lemma refine_tupleAgree_refl_True :
+    forall (h : Heading)
+           (tup : @Tuple h)
+           (attrlist attrlist' : list (Attributes h)),
+      refine {b |
+              decides b (tupleAgree tup tup attrlist'
+                         -> tupleAgree tup tup attrlist)}
+             (ret true).
+  Proof.
+    unfold refine; intros; inversion_by computes_to_inv.
+    subst; econstructor; simpl; auto using tupleAgree_refl.
+  Qed.
