ADTExamples/QueryStructure/GeneralQueryRefinements.v
@@ -1,0 +1,67 @@
+Require Import String Omega List FunctionalExtensionality Ensembles
+        Computation ADT ADTRefinement ADTNotation QueryStructureSchema
+        QueryQSSpecs QueryStructure.
+
+Definition Equivalent_Ensembles {A : Type}
+           (P Q : Ensemble A) := forall a, P a <-> Q a.
+
+  Lemma Equivalent_Swap_In {A}
+        (qs : QueryStructureHint) (R R' : _)
+        (bod : Tuple -> Tuple -> Ensemble A)
+  :
+    Equivalent_Ensembles
+      (@Query_In qs _ R (fun tup => @Query_In qs _ R' (bod tup)))
+      (@Query_In qs _ R' (fun tup => @Query_In qs _ R
+                                               (fun tup' => bod tup' tup))).
+  Proof.
+    unfold Equivalent_Ensembles, Query_In; split; intros;
+    repeat (progress (destruct_ex; intuition)); eexists;
+    split; eauto.
+  Qed.
+
+  Lemma Equivalent_Swap_In_Where {A}
+        (qs : QueryStructureHint) (R : _)
+        {heading}
+        (bod : @Tuple heading -> Tuple -> Ensemble A)
+        (P : @Tuple heading -> Prop)
+  :
+    pointwise_relation
+      Tuple Equivalent_Ensembles
+      (fun tup' : Tuple =>
+         (@Query_In qs _ R
+                    (fun tup => Query_Where (P tup') (bod tup' tup))))
+      (fun tup' : Tuple =>
+         Query_Where (P tup') (@Query_In qs _ R (bod tup'))).
+  Proof.
+    unfold Equivalent_Ensembles, Query_In, Query_Where; split; intros;
+    repeat (progress (destruct_ex; intuition)); eexists;
+    split; eauto.
+  Qed.
+
+  Add Parametric Morphism {A: Type} :
+    (Query_For)
+      with signature (@Equivalent_Ensembles A ==> refine)
+        as refine_Query_For_Equivalent.
+  Proof.
+    unfold impl, Query_For, refine; intros.
+    inversion_by computes_to_inv.
+    econstructor; split_iff; split; intros; eauto.
+    apply H; apply H1; auto.
+    apply H2; apply H; auto.
+  Qed.
+
+  Add Parametric Morphism {A: Type}
+      (qs : QueryStructureHint) (R : _)
+  :
+    (fun bod => Query_For (@Query_In qs _ R bod))
+      with signature ((pointwise_relation Tuple (@Equivalent_Ensembles A) ==> refine ))
+        as refine_Query_For_In_Equivalent.
+  Proof.
+    unfold impl, Query_For, pointwise_relation, Query_In, In, refine.
+    intros; inversion_by computes_to_inv.
+    econstructor; split_iff; split; intros; eauto.
+    destruct (H1 _ H0); eexists; intuition; eauto.
+    apply H; auto.
+    destruct_ex; apply H2; eexists; intuition; eauto.
+    apply H; auto.
+  Qed.
