ADTExamples/QueryStructure/ListInsertRefinements.v
@@ -1,0 +1,96 @@
+Require Import String Omega List FunctionalExtensionality Ensembles
+        Computation ADT ADTRefinement ADTNotation QueryStructureSchema
+        QueryQSSpecs InsertQSSpecs QueryStructure ProcessScheduler.AdditionalLemmas.
+
+Definition decideable_Heading_Domain
+             (h : Heading) :=
+    forall (idx : Attributes h)
+           (t t' : Domain h idx), {t = t'} + {t <> t'}.
+
+  Fixpoint Tuple_Agree_dec
+             (h : Heading)
+             (h_dec_eq : decideable_Heading_Domain h)
+             (attrlist : list (Attributes h))
+  : forall (tup tup' : Tuple),
+      {tupleAgree tup tup' attrlist} + {~tupleAgree tup tup' attrlist}.
+  Proof.
+  Admitted.
+
+  Fixpoint Check_List_Prop {A}
+           (cond : A -> bool)
+           (l : list A)
+  : bool :=
+    match l with
+        | [] => true
+        | a :: l' => if (cond a) then
+                          Check_List_Prop cond l'
+                        else false
+    end.
+
+  Definition In_List_Key
+           (h : Heading)
+           (h_dec_eq : decideable_Heading_Domain h)
+           (attrlist : list (Attributes h))
+           (tup : Tuple)
+           (l : list Tuple) :=
+    Check_List_Prop (fun tup' =>
+                       if (Tuple_Agree_dec h_dec_eq attrlist tup tup')
+                       then true
+                       else false) l.
+
+  Lemma refine_unused_key_check
+  : forall (h : Heading)
+           (h_dec_eq : decideable_Heading_Domain h)
+           (attrlist attrlist' : list (Attributes h))
+           (tup : Tuple)
+           (rel : Ensemble Tuple)
+           (l : list Tuple),
+      EnsembleListEquivalence rel l
+      -> refine {b | decides b
+                             (forall tup' : Tuple,
+                                rel tup' ->
+                                tupleAgree tup tup' attrlist' ->
+                                tupleAgree tup tup' attrlist)}
+                (ret (In_List_Key h_dec_eq attrlist tup l)).
+  Admitted.
+
+  Lemma refine_unused_key_check'
+  : forall (h : Heading)
+           (h_dec_eq : decideable_Heading_Domain h)
+           (attrlist attrlist' : list (Attributes h))
+           (tup : Tuple)
+           (rel : Ensemble Tuple)
+           (l : list Tuple),
+      EnsembleListEquivalence rel l
+      -> refine {b | decides b
+                             (forall tup' : Tuple,
+                                rel tup' ->
+                                tupleAgree tup' tup attrlist' ->
+                                tupleAgree tup' tup attrlist)}
+                (ret (In_List_Key h_dec_eq attrlist tup l)).
+  Admitted.
+
+  Lemma refine_foreign_key_check
+  : forall (h : Heading)
+           (rel : Ensemble Tuple)
+           (l : list Tuple)
+           (P : Ensemble Tuple)
+           (cond : Tuple -> bool),
+      EnsembleListEquivalence rel l
+      -> refine {b  |
+                 decides b
+                         (exists tup' : @Tuple h,
+                            rel tup' /\
+                            P tup')}
+                (ret (Check_List_Prop cond l)).
+    Admitted.
+
+      Add Parametric Morphism {A: Type} (b : bool):
+        (If_Then_Else b)
+          with signature (
+            @refine A ==> @refine A ==> refine)
+            as refine_refine_if.
+      Proof.
+        unfold refine, If_Then_Else; intros.
+        destruct b; eauto.
+      Qed.
