ADTExamples/QueryStructure/ProcessScheduler.v
@@ -42,7 +42,7 @@ Section ProcessSchedulerExample.
   Definition Process := (Tuple ProcessSchema).
 
   Definition SPAWN     := "Spawn".
-  Definition ENUMERATE := "Enumerate".
+  Definition ENUMERATE := "Enumerate".q
   Definition COUNT     := "Count".
 
   Definition ProcessSchedulerSig := ADTsignature {
@@ -58,19 +58,19 @@ Section ProcessSchedulerExample.
 
   Local Open Scope Tuple_scope.
 
-  Definition ProcessSchedulerSpec : ADT ProcessSchedulerSig := 
-    QueryADTRep 
+  Definition ProcessSchedulerSpec : ADT ProcessSchedulerSig :=
+    QueryADTRep
       ProcessSchedulerRefRep {
         def update SPAWN (ns : nat) : rep := (* TODO: pid/0 *)
           Insert <NS: ns, PID: 0, STATE: Sleeping, CPU: 0> into PROCESSES_TABLE;
-          
+
         def query ENUMERATE (state : State) : list (prod nat nat) :=
           For (p in PROCESSES_TABLE)
               Where (p!STATE == state)
               Return (p!NS, p!PID)(*,
-          
+
         def query COUNT (_: unit) : nat :=
-          Count (For (p in PROCESSES_TABLE) 
+          Count (For (p in PROCESSES_TABLE)
                  Return 1)*)
       }.
 
@@ -87,29 +87,29 @@ Section ProcessSchedulerExample.
 
   Definition ExtractNSAndPID (processes : list Process) :=
     map (fun p => (p!NS, p!PID)) processes.
-  
+
   Definition SimpleDB_equivalence (rep: ProcessSchedulerRefRep) (db: SimpleDB) :=
     (GetRelation rep PROCESSES_TABLE) = db.
 
   Definition SimpleDB_enumerate db state :=
-    ret (ExtractNSAndPID  
+    ret (ExtractNSAndPID
            (filter (fun (p: Process) => beq_state p!STATE state) db)).
 
   Definition SimpleDB_spawn (db: list Process) (ns: nat) :=
     ret (<NS: ns, PID: 0, STATE: Sleeping, CPU: 0> :: db).
 
-  Lemma eq_ret_compute : 
+  Lemma eq_ret_compute :
     forall (A: Type) (x y: A), x = y -> ret x ↝ y.
   Proof.
     intros; subst; apply ReturnComputes; trivial.
   Qed.
 
-  Lemma eq_indistinguishable : 
-    forall {A: Type} (l1 l2: list A), l1 = l2 -> indistinguishable l1 l2. 
+  Lemma eq_indistinguishable :
+    forall {A: Type} (l1 l2: list A), l1 = l2 -> indistinguishable l1 l2.
   Proof.
     intros A l1 l2 eq12; unfold indistinguishable; subst l2; induction l1; [apply perm_nil | apply perm_skip]; trivial.
   Qed.
-  
+
   Ltac rinse func param_name :=
     intros r_o newrep param_name eq_ro_newrep;
     subst r_o;
@@ -123,7 +123,7 @@ Section ProcessSchedulerExample.
     Sharpened ProcessSchedulerSpec.
   Proof.
     hone representation' using SimpleDB_equivalence.
-    
+
     hone' observer ENUMERATE using SimpleDB_enumerate;
       [ rinse SimpleDB_enumerate state | ].
 
@@ -136,7 +136,7 @@ Section ProcessSchedulerExample.
 
     apply eq_indistinguishable.
 
-    induction newrep as [ | head tail IH]; 
+    induction newrep as [ | head tail IH];
       simpl in *;
       [ | rewrite <- IH;
           destruct (head!(STATE)), state;
@@ -151,10 +151,10 @@ Section ProcessSchedulerExample.
 
     intros oldrep oldrep_equiv_newrep.
 
-    Definition rels_builder (db: SimpleDB) _constr_ : 
+    Definition rels_builder (db: SimpleDB) _constr_ :
       ilist (fun ns : NamedSchema => Relation (relSchema ns))
             (qschemaSchemas ProcessSchedulerSchema) :=
-      icons (B := fun ns => Relation (relSchema ns)) _ 
+      icons (B := fun ns => Relation (relSchema ns)) _
             {| rel := db; constr := _constr_ |} (inil _).
 
     Definition ref_rep_builder db _constr_ _crossConstr_ : QueryStructure ProcessSchedulerSchema :=
@@ -180,9 +180,9 @@ Section ProcessSchedulerExample.
     finish sharpening.
 
     Grab Existential Variables.
-    
+
     simpl; trivial.
-    
+
     intros; simpl in *. (* TODO: Verify this. Shouldn't tup2 be in <...> :: newrep as well? *)
     (*
       unfold tupleAgree; simpl. intros. simpl in H.
@@ -190,55 +190,55 @@ Section ProcessSchedulerExample.
       destruct H1; subst; simpl in H0.
     *)
   Admitted.
-  
+
   Inductive BinaryTree :=
   | Empty : BinaryTree
   | Leaf : Process -> BinaryTree
   | Branch : BinaryTree -> BinaryTree -> BinaryTree.
-  
+
   Fixpoint InTree process tree :=
     match tree with
       | Empty => False
       | Leaf p => process = p
       | Branch lbranch rbranch => InTree process lbranch \/ InTree process rbranch
     end.
-  
+
   Fixpoint IsSearchTree tree :=
     match tree with
       | Empty => True
       | Leaf _ => True
-      | Branch lbranch rbranch => 
-        IsSearchTree lbranch 
+      | Branch lbranch rbranch =>
+        IsSearchTree lbranch
         /\ IsSearchTree rbranch
         /\ (forall (procl procr : Process),
-              InTree procl lbranch -> 
+              InTree procl lbranch ->
               InTree procr rbranch ->
               le procl!PID procr!PID)
     end.
-  
+
   (* TODO: Look at fmap *)
-  
+
   Fixpoint ValuesMatch (*prop*) value tree :=
     match tree with
       | Empty => True
       | Leaf p => p!STATE = value
       | Branch lbranch rbranch => ValuesMatch (*prop*) value lbranch /\ ValuesMatch (*prop*) value rbranch
     end.
-  
-  Definition SortedDB_table state := 
+
+  Definition SortedDB_table state :=
     sig (fun table : BinaryTree => ValuesMatch state table /\ IsSearchTree table).
-  
+
   Definition SortedDB := prod (SortedDB_table Running) (SortedDB_table Sleeping).
-  
+
   Definition ExtractTree {state : State} (table : SortedDB_table state) := proj1_sig table.
-  
+
   Fixpoint Flatten tree :=
     match tree with
       | Empty => []
       | Leaf l => [l]
       | Branch lbranch rbranch => (Flatten lbranch ++ Flatten rbranch) % list
     end.
-  
+
   Check sig.
 
   Definition ExtractCorrespondingTree (state: State) (db: SortedDB) :=
@@ -251,14 +251,14 @@ Section ProcessSchedulerExample.
 
   Definition InDB x db :=
     InTree x (ExtractCorrespondingTree x!STATE db).
-  
+
   Definition SortedDB_enumerate (db : SortedDB) state :=
     ret (ExtractNSAndPID (Flatten (ExtractCorrespondingTree state db))).
 
   Definition SortedDB_equivalence (ref: ProcessSchedulerRefRep) (db : SortedDB) :=
     forall x, List.In x (GetRelation ref PROCESSES_TABLE) <-> InDB x db.
 
-  Lemma sharpened_btree : 
+  Lemma sharpened_btree :
     Sharpened ProcessSchedulerSpec.
   Proof.
     hone representation' using SortedDB_equivalence.
@@ -270,11 +270,11 @@ Section ProcessSchedulerExample.
       constructor 3;
       intros oldrep oldrep_equiv_newrep;
       constructor.
-    
+
     unfold ExtractNSAndPID, Flatten, ExtractCorrespondingTree; destruct state, newrep; simpl.
- 
+
     (*
-      Lemma lists_without_elements_are_empty: 
+      Lemma lists_without_elements_are_empty:
         forall (A: Type) (lst: list A), (forall item, List.In item lst <-> False) -> lst = [].
       Proof.
         intros A lst H; destruct lst as [|a]; intuition.
