ADTExamples/QueryStructure/Relation.v
@@ -6,13 +6,13 @@ Require Import List String FunctionalExtensionality Ensembles
    which satisfy the schema constraints. *)
 
 Record Relation (RelationSchema : Schema) :=
-  { rel : Ensemble (Tuple (schemaHeading RelationSchema));
+  { rel : Ensemble (@Tuple (schemaHeading RelationSchema));
     constr :
       forall tup tup',
-        rel tup -> 
-        rel tup' -> 
+        rel tup ->
+        rel tup' ->
         schemaConstraints RelationSchema tup tup'
   }.
 
 Definition UnConstrRelation (RelationSchema : Schema) :=
-  Ensemble (Tuple (schemaHeading RelationSchema)).
+  Ensemble (@Tuple (schemaHeading RelationSchema)).
