ADTRefinement/GeneralBuildADTRefinements.v
@@ -19,7 +19,7 @@ Section BuildADTRefinements.
             (obsSigs : list obsSig)
             (mutDefs : ilist (@mutDef Rep) mutSigs)
             (obsDefs : ilist (@obsDef Rep) obsSigs)
-            (idx : BoundedString (List.map mutID mutSigs))
+            (idx : @BoundedString (List.map mutID mutSigs))
             (newDef : mutDef (nth_Bounded mutID mutSigs idx))
   :
     (forall mutIdx,
@@ -45,7 +45,7 @@ Section BuildADTRefinements.
             (obsSigs : list obsSig)
             (mutDefs : ilist (@mutDef Rep) mutSigs)
             (obsDefs : ilist (@obsDef Rep) obsSigs)
-            (idx : BoundedString (List.map mutID mutSigs))
+            (idx : @BoundedString (List.map mutID mutSigs))
             (newDef : mutDef (nth_Bounded mutID mutSigs idx))
   :
     refineMutator eq
@@ -59,29 +59,27 @@ Section BuildADTRefinements.
     simpl; unfold refine; intros; subst; eauto.
   Qed.
 
-  Corollary refineADT_BuildADT_refinement_of_Mutator_eq
+  Corollary SharpenStep_BuildADT_ReplaceMutator_eq
             (Rep : Type)
-            (SiR : Rep -> Rep -> Prop)
             (mutSigs : list mutSig)
             (obsSigs : list obsSig)
             (mutDefs : ilist (@mutDef Rep) mutSigs)
             (obsDefs : ilist (@obsDef Rep) obsSigs)
-            (idx : BoundedString (List.map mutID mutSigs))
+            (idx : @BoundedString (List.map mutID mutSigs))
+            (newDef : mutDef (nth_Bounded mutID mutSigs idx))
   :
-    forall
-      (ref : forall r_n n,
-               Refinement
-                 of
-                 (r_o' <- (mutBody (ith_Bounded _ mutDefs idx)) r_n n;
-                  {r_n0 : Rep | r_o' = r_n0})%comp),
-      refineADT
-        (BuildADT mutDefs obsDefs)
-        (ADTReplaceMutDef mutDefs obsDefs idx
-                          {| mutBody := fun r_n n => proj1_sig (ref r_n n) |} ).
+    (forall r_n n,
+      refine (mutBody (ith_Bounded mutID mutDefs idx) r_n n) (mutBody newDef r_n n))
+    -> Sharpened (ADTReplaceMutDef mutDefs obsDefs idx newDef)
+    -> Sharpened (BuildADT mutDefs obsDefs).
   Proof.
-    intros; eapply refineADT_BuildADT_ReplaceMutator_eq.
-    simpl; intros; subst; eapply (proj2_sig (ref r_n n)).
-  Qed.
+    intros; eapply SharpenStep; eauto.
+    destruct newDef; simpl.
+    intros; eapply refineADT_BuildADT_ReplaceMutator_eq;
+    simpl; intros; subst; try reflexivity;
+    setoid_rewrite refineEquiv_pick_eq'; simplify with monad laws;
+    eauto.
+  Defined.
 
   Lemma refineADT_BuildADT_ReplaceMutator_sigma
         (RepT : Type)
@@ -91,7 +89,7 @@ Section BuildADTRefinements.
         (obsSigs : list obsSig)
         (mutDefs : ilist (@mutDef (sig RepInv)) mutSigs)
         (obsDefs : ilist (@obsDef (sig RepInv)) obsSigs)
-        (idx : BoundedString (List.map mutID mutSigs))
+        (idx : @BoundedString (List.map mutID mutSigs))
         (newDef : mutDef (nth_Bounded mutID mutSigs idx))
   : refineMutator (fun x y => proj1_sig x = proj1_sig y)
                   (mutBody (ith_Bounded _ mutDefs idx))
@@ -117,7 +115,7 @@ Section BuildADTRefinements.
             (obsSigs : list obsSig)
             (mutDefs : ilist (@mutDef Rep) mutSigs)
             (obsDefs : ilist (@obsDef Rep) obsSigs)
-            (idx : BoundedString (List.map obsID obsSigs))
+            (idx : @BoundedString (List.map obsID obsSigs))
             (newDef : obsDef (nth_Bounded _ obsSigs idx))
             SiR
             (SiR_reflexive_mutator : forall mutIdx,
@@ -137,14 +135,13 @@ Section BuildADTRefinements.
     eapply ith_replace_BoundedIndex_ind; eauto.
   Qed.
 
-
   Lemma refineADT_BuildADT_ReplaceObserver_eq
             (Rep : Type)
             (mutSigs : list mutSig)
             (obsSigs : list obsSig)
             (mutDefs : ilist (@mutDef Rep) mutSigs)
             (obsDefs : ilist (@obsDef Rep) obsSigs)
-            (idx : BoundedString (List.map obsID obsSigs))
+            (idx : @BoundedString (List.map obsID obsSigs))
             (newDef : obsDef (nth_Bounded _ obsSigs idx))
   : refineObserver eq
                    (obsBody (ith_Bounded _ obsDefs idx))
@@ -157,6 +154,29 @@ Section BuildADTRefinements.
     reflexivity.
   Qed.
 
+  Corollary SharpenStep_BuildADT_ReplaceObserver_eq
+            (Rep : Type)
+            (mutSigs : list mutSig)
+            (obsSigs : list obsSig)
+            (mutDefs : ilist (@mutDef Rep) mutSigs)
+            (obsDefs : ilist (@obsDef Rep) obsSigs)
+            (idx : @BoundedString (List.map obsID obsSigs))
+            (newDef : obsDef (nth_Bounded _ obsSigs idx))
+  :
+    (forall r_n n,
+      refine (obsBody (ith_Bounded obsID obsDefs idx) r_n n) (obsBody newDef r_n n))
+    -> Sharpened (ADTReplaceObsDef mutDefs obsDefs idx newDef)
+    -> Sharpened (BuildADT mutDefs obsDefs).
+  Proof.
+    intros; eapply SharpenStep; eauto.
+    destruct newDef; simpl.
+    intros; eapply refineADT_BuildADT_ReplaceObserver_eq;
+    simpl; intros; subst; try reflexivity;
+    simplify with monad laws; eauto.
+  Qed.
+
+
+
   Lemma refineADT_BuildADT_ReplaceObserver_sigma
         (RepT : Type)
         (RepInv : RepT -> Prop)
@@ -164,7 +184,7 @@ Section BuildADTRefinements.
         (obsSigs : list obsSig)
         (mutDefs : ilist (@mutDef (sig RepInv)) mutSigs)
         (obsDefs : ilist (@obsDef (sig RepInv)) obsSigs)
-        (idx : BoundedString (List.map obsID obsSigs))
+        (idx : @BoundedString (List.map obsID obsSigs))
         (newDef : obsDef (nth_Bounded _ obsSigs idx))
   : refineObserver (fun x y => proj1_sig x = proj1_sig y)
                    (obsBody (ith_Bounded _ obsDefs idx))
@@ -273,6 +293,89 @@ Tactic Notation "hone'" "mutator" constr(mutIdx) :=
   [set_evars;
     simpl in *; intros; subst;
     autosetoid_rewrite with refine_monad | ].
+
+  Tactic Notation "hone" "mutator" constr(mutIdx) :=
+    let A :=
+        match goal with
+            |- Sharpened ?A => constr:(A) end in
+    let ASig := match type of A with
+                    ADT ?Sig => Sig
+                end in
+    let mutSigs :=
+        match ASig with
+            BuildADTSig ?mutSigs _ => constr:(mutSigs) end in
+    let obsSigs :=
+        match ASig with
+            BuildADTSig _ ?obsSigs => constr:(obsSigs) end in
+    let mutDefs :=
+        match A with
+            BuildADT ?mutDefs _  => constr:(mutDefs) end in
+    let obsDefs :=
+        match A with
+            BuildADT _ ?obsDefs  => constr:(obsDefs) end in
+    let Rep' :=
+        match A with
+            @BuildADT ?Rep _ _ _ _ => constr:(Rep) end in
+    let MutatorIndex' := eval simpl in (MutatorIndex ASig) in
+    let ObserverIndex' := eval simpl in (ObserverIndex ASig) in
+    let MutatorDom' := eval simpl in (MutatorDom ASig) in
+    let mutIdxB := eval simpl in
+    (@Build_BoundedIndex _ (List.map mutID mutSigs) mutIdx _) in
+        eapply (@SharpenStep_BuildADT_ReplaceMutator_eq
+                 Rep'  _ _ mutDefs obsDefs mutIdxB
+                 (@Build_mutDef Rep'
+                                {| mutID := mutIdx;
+                                   mutDom := MutatorDom' mutIdxB
+                                |}
+                                _
+               ));
+      [ intros; try (apply refine_pick_forall_Prop with
+                     (P := fun r_n n r_o => _); intros) |
+          cbv beta in *; simpl in *;
+          cbv beta delta [replace_BoundedIndex replace_Index] in *;
+          simpl in *].
+
+  Tactic Notation "hone" "observer" constr(obsIdx) :=
+    let A :=
+        match goal with
+            |- Sharpened ?A => constr:(A) end in
+    let ASig := match type of A with
+                    ADT ?Sig => Sig
+                end in
+    let mutSigs :=
+        match ASig with
+            BuildADTSig ?mutSigs _ => constr:(mutSigs) end in
+    let obsSigs :=
+        match ASig with
+            BuildADTSig _ ?obsSigs => constr:(obsSigs) end in
+    let mutDefs :=
+        match A with
+            BuildADT ?mutDefs _  => constr:(mutDefs) end in
+    let obsDefs :=
+        match A with
+            BuildADT _ ?obsDefs  => constr:(obsDefs) end in
+    let Rep' :=
+        match A with
+            @BuildADT ?Rep _ _ _ _ => constr:(Rep) end in
+    let MutatorIndex' := eval simpl in (MutatorIndex ASig) in
+    let ObserverIndex' := eval simpl in (ObserverIndex ASig) in
+    let ObserverDomCod' := eval simpl in (ObserverDomCod ASig) in
+    let obsIdxB := eval simpl in
+    (@Build_BoundedIndex _ (List.map obsID obsSigs) obsIdx _) in
+        eapply (@SharpenStep_BuildADT_ReplaceObserver_eq
+                  Rep'  _ _ mutDefs obsDefs obsIdxB
+                  (@Build_obsDef Rep'
+                                 {| obsID := obsIdx;
+                                    obsDom := fst (ObserverDomCod' obsIdxB);
+                                    obsCod := snd (ObserverDomCod' obsIdxB)
+                                 |}
+                                 _
+                                ));
+          [ intros; try (apply refine_pick_forall_Prop with
+                         (P := fun r_n n r_o => _); intros) |
+            cbv beta in *; simpl in *;
+            cbv beta delta [replace_BoundedIndex replace_Index] in *;
+            simpl in *].
 
 Tactic Notation "finish" "honing" :=
   subst_body;
